verif/SplitAtA.v
@@ -1,0 +1,41 @@
+Require Import List.
+Import ListNotations.
+Require Import String.
+
+(* Borrow from CompCert *)
+Require Import Coqlib.
+Require Import Bitvectors.
+
+Require Import AST.
+Require Import Semantics.
+Require Import Utils.
+Require Import Builtins.
+Require Import BuiltinSem.
+Require Import Values.        
+
+Require Import EvalTac.
+
+Import HaskellListNotations.
+Open Scope string.
+
+Require Import SplitAt.
+
+Lemma eval_a :
+  exists v,
+    eval_expr ge empty (EVar a) v /\ force_list ge empty v (@from_bitv 8 (@repr 8 1)).
+Proof.
+  eexists; split.
+  e. e. e. e. e. e. e.
+  e. e. e. e. e. e. e. e. e. e. e.
+  e. e. e. e. e. e. e. g.
+  e. e. e. e. e. e. e. e. e. e. e. e. g.
+  repeat e.
+  e. (* TODO: implement splitAt semantics *)
+  e. repeat e.
+  e. e. e. e.
+  e. e. e. e.
+  e. e. e. e. g.
+  e. e. e. e. e. e. e. e. e. e.
+  e. e. e. e. e.
+  e. repeat e. repeat e. 
+Qed.
